src/riscv/Platform/MetricMaterializeRiscvProgram.v
@@ -39,7 +39,7 @@ Section Riscv.
     endCycleEarly A := act (addMetricInstructions 1, EndCycleEarly A) ret;
   |}.
 
-  Global Instance MetricMaterializeWithLeakage : RiscvProgramWithLeakage := {|
+  Global Instance MetricMaterializeWithLeakage : RiscvProgramWithLeakage (free action result) word := {|
     RVP := MetricMaterialize;
     leakEvent a := act (id, LeakEvent a) ret
   |}.
