src/riscv/Spec/MetricPrimitives.v
@@ -21,8 +21,8 @@ Section MetricPrimitives.
 
   Context {M: Type -> Type}.
   Context {MM: Monad M}.
-  Context {RVM: RiscvProgramWithLeakage}.
-  Context {RVS: @RiscvMachine M word _ _ RVM.(RVP)}.
+  Context {RVM: RiscvProgramWithLeakage M word}.
+  Context {RVS: @RiscvMachine M word _ _ RVM}.
 
   (* monadic computations used for specifying the behavior of RiscvMachines should be "sane"
      in the sense that we never step to the empty set (that's not absence of failure, since
@@ -110,15 +110,15 @@ Section MetricPrimitives.
        x = Register0 /\ post tt initialL) ->
       mcomp_sat (setRegister x v) initialL post;
 
-    spec_loadByte: spec_load 1 (Machine.loadByte (RiscvProgram := RVM.(RVP))) Memory.loadByte;
-    spec_loadHalf: spec_load 2 (Machine.loadHalf (RiscvProgram := RVM.(RVP))) Memory.loadHalf;
-    spec_loadWord: spec_load 4 (Machine.loadWord (RiscvProgram := RVM.(RVP))) Memory.loadWord;
-    spec_loadDouble: spec_load 8 (Machine.loadDouble (RiscvProgram := RVM.(RVP))) Memory.loadDouble;
+    spec_loadByte: spec_load 1 (Machine.loadByte (RiscvProgram := RVM)) Memory.loadByte;
+    spec_loadHalf: spec_load 2 (Machine.loadHalf (RiscvProgram := RVM)) Memory.loadHalf;
+    spec_loadWord: spec_load 4 (Machine.loadWord (RiscvProgram := RVM)) Memory.loadWord;
+    spec_loadDouble: spec_load 8 (Machine.loadDouble (RiscvProgram := RVM)) Memory.loadDouble;
 
-    spec_storeByte: spec_store 1 (Machine.storeByte (RiscvProgram := RVM.(RVP))) Memory.storeByte;
-    spec_storeHalf: spec_store 2 (Machine.storeHalf (RiscvProgram := RVM.(RVP))) Memory.storeHalf;
-    spec_storeWord: spec_store 4 (Machine.storeWord (RiscvProgram := RVM.(RVP))) Memory.storeWord;
-    spec_storeDouble: spec_store 8 (Machine.storeDouble (RiscvProgram := RVM.(RVP))) Memory.storeDouble;
+    spec_storeByte: spec_store 1 (Machine.storeByte (RiscvProgram := RVM)) Memory.storeByte;
+    spec_storeHalf: spec_store 2 (Machine.storeHalf (RiscvProgram := RVM)) Memory.storeHalf;
+    spec_storeWord: spec_store 4 (Machine.storeWord (RiscvProgram := RVM)) Memory.storeWord;
+    spec_storeDouble: spec_store 8 (Machine.storeDouble (RiscvProgram := RVM)) Memory.storeDouble;
 
     spec_getPC: forall (initialL: MetricRiscvMachine) (post: word -> MetricRiscvMachine -> Prop),
         post initialL.(getPc) initialL ->
